Core/Protocol.v
@@ -1,0 +1,615 @@
+From mathcomp.ssreflect
+Require Import ssreflect ssrbool ssrnat eqtype ssrfun seq fintype.
+From mathcomp
+Require Import path.
+Require Import Eqdep Relations.
+From HTT
+Require Import pred prelude idynamic ordtype pcm finmap unionmap heap.
+From CasperToychain
+Require Import Blockforest.
+Set Implicit Arguments.
+Unset Strict Implicit.
+Unset Printing Implicit Defensive.
+
+(* ------------------*)
+(* PROTOCOL MESSAGES *)
+(* ------------------*)
+
+Definition peers_t := seq Address.
+
+Inductive Message :=
+| BlockMsg of block
+| TxMsg of Transaction
+| InvMsg of seq Hash
+| GetDataMsg of Hash.
+
+Inductive InternalTransition :=
+  | TxT of Transaction
+  | MintT.
+
+Definition eq_msg a b :=
+ match a, b with
+  | BlockMsg bA, BlockMsg bB => (bA == bB)
+  | BlockMsg _, _ => false
+  | TxMsg tA, TxMsg tB => (tA == tB)
+  | TxMsg _, _ => false
+  | InvMsg hA, InvMsg hB => (hA == hB)
+  | InvMsg _, _ => false
+  | GetDataMsg hA, GetDataMsg hB => (hA == hB)
+  | GetDataMsg _, _ => false
+ end.
+
+Ltac simple_tactic mb n n' B :=
+  (case: mb=>//[b'|t'|p'|p']; do? [by constructor 2];
+   case B: (n == n'); [by case/eqP:B=><-; constructor 1|constructor 2];
+   case=>E; subst n'; rewrite eqxx in B).
+
+Lemma eq_msgP : Equality.axiom eq_msg.
+Proof.
+move=> ma mb. rewrite/eq_msg.
+case: ma=>[b|t|h|h].
+- case:mb=>////[b'|t'|h'|h']; do? [by constructor 2].
+  case B: (b == b'); [by case/eqP:B=><-; constructor 1|constructor 2].
+  by case=>Z; subst b'; rewrite eqxx in B.
+- case:mb=>////[b'|t'|h'|h']; do? [by constructor 2].
+  case B: (t == t'); [by case/eqP:B=><-; constructor 1|constructor 2].
+  by case=>Z; subst t'; rewrite eqxx in B.
+- case:mb=>////[b'|t'|h'|h']; do? [by constructor 2].
+  case B: (h == h'); [by case/eqP:B=><-; constructor 1|constructor 2].
+  by case=>Z; subst h'; rewrite eqxx in B.
+- case:mb=>////[b'|t'|h'|h']; do? [by constructor 2].
+  case B: (h == h'); [by case/eqP:B=><-; constructor 1|constructor 2].
+  by case=>Z; subst h'; rewrite eqxx in B.
+Qed.
+  
+Canonical Msg_eqMixin := Eval hnf in EqMixin eq_msgP.
+Canonical Msg_eqType := Eval hnf in EqType Message Msg_eqMixin.
+
+Record Packet := mkP {src: Address; dst: Address; msg: Message}.
+
+Definition eq_pkt a b :=
+  ((src a) == (src b)) && ((dst a) == (dst b)) && ((msg a) == (msg b)).
+
+Lemma eq_pktP : Equality.axiom eq_pkt.
+Proof.
+case=>sa da ma [sb] db mb; rewrite/eq_pkt/=.
+case P1: (sa == sb)=>/=; last by constructor 2; case=>/eqP; rewrite P1.
+case P2: (da == db)=>/=; last by constructor 2; case=> _ /eqP; rewrite P2.
+case P3: (ma == mb)=>/=; last by constructor 2; case=> _ _ /eqP; rewrite P3.
+by constructor 1; move/eqP: P1=><-; move/eqP: P2=><-; move/eqP: P3=><-.
+Qed.
+
+Canonical Packet_eqMixin := Eval hnf in EqMixin eq_pktP.
+Canonical Packet_eqType := Eval hnf in EqType Packet Packet_eqMixin.
+
+Definition ToSend := seq Packet.
+Definition emitZero : ToSend := [::].
+Definition emitOne (packet : Packet) : ToSend := [:: packet].
+Definition emitMany (packets : ToSend) := packets.
+
+Definition emitBroadcast (from : Address) (dst : seq Address) (msg : Message) :=
+  [seq (mkP from to msg) | to <- dst].
+
+(* ------------------*)
+(* NODE STATE & CODE *)
+(* ------------------*)
+
+Record State :=
+  Node {
+    id : Address;
+    peers : peers_t;
+    blockTree : Blockforest;
+    txPool : TxPool;
+  }.
+
+Definition Init (n : Address) : State :=
+  Node n [:: n] (#GenesisBlock \\-> GenesisBlock) [::].
+
+Lemma peers_uniq_init (n : Address) : uniq [::n].
+Proof. by []. Qed.
+
+Definition procMsg (st: State) (from : Address) (msg: Message) (ts: Timestamp) :=
+    let: Node n prs bt pool := st in
+    match msg with
+    | BlockMsg b =>
+      let: newBt := btExtend bt b in
+      let: newPool := [seq t <- pool | txValid t (btChain newBt)] in
+      let: ownHashes := (keys_of newBt) ++ [seq hashT t | t <- newPool] in
+      pair (Node n prs newBt newPool) (emitBroadcast n prs (InvMsg ownHashes))
+
+    | TxMsg tx =>
+      let: newPool := tpExtend pool bt tx in
+      let: ownHashes := (keys_of bt) ++ [seq hashT t | t <- newPool] in
+      pair (Node n prs bt newPool) (emitBroadcast n prs (InvMsg ownHashes))
+
+    | InvMsg peerHashes =>
+      let: ownHashes := (keys_of bt) ++ [seq hashT t | t <- pool] in
+      let: newH := [seq h <- peerHashes | h \notin ownHashes] in
+      let: gets := [seq mkP n from (GetDataMsg h) | h <- newH] in
+      pair st (emitMany gets)
+
+    | GetDataMsg h =>
+      (* Do not respond to yourself *)
+      if from == n then pair st emitZero else
+      let: matchingBlocks := [seq b <- [:: get_block bt h] | b != GenesisBlock] in
+      match ohead matchingBlocks with
+      | Some b => pair (Node n prs bt pool) (emitOne (mkP n from (BlockMsg b)))
+      | None =>
+        let: matchingTxs := [seq t <- pool | (hashT t) == h] in
+        match ohead matchingTxs with
+        | Some tx =>
+          pair (Node n prs bt pool) (emitOne (mkP n from (TxMsg tx)))
+        | None => pair st emitZero
+        end
+      end
+    end.
+
+Definition procInt (st : State) (tr : InternalTransition) (ts : Timestamp) :=
+    let: Node n prs bt pool := st in
+    match tr with
+    | TxT tx => pair st (emitBroadcast n prs (TxMsg tx))
+
+    (* Assumption: nodes broadcast to themselves as well! => simplifies logic *)
+    | MintT =>
+      let: bc := btChain bt in
+      let: allowedTxs := [seq t <- pool | txValid t bc] in
+      match genProof n bc allowedTxs ts with
+      | Some pf =>
+        if VAF pf ts bc allowedTxs then
+          let: prevBlock := last GenesisBlock bc in
+          let: block := mkB (hashB prevBlock) allowedTxs pf in
+          if tx_valid_block bc block then
+            let: newBt := btExtend bt block in
+            let: newPool := [seq t <- pool | txValid t (btChain newBt)] in
+            let: ownHashes := (keys_of newBt) ++ [seq hashT t | t <- newPool] in
+            pair (Node n prs newBt newPool) (emitBroadcast n prs (BlockMsg block))
+          else
+            pair st emitZero
+        else
+          pair st emitZero
+      | None => pair st emitZero
+      end
+    end.
+
+Definition Address_ordMixin := fin_ordMixin Address.
+Canonical Address_ordType := Eval hnf in OrdType Address Address_ordMixin.
+
+Definition StateMap := union_map [ordType of Address] State.
+
+Definition initState' s : StateMap := foldr (fun a m => (a \\-> Init a) \+ m) Unit s.
+
+(* Master-lemma, proving a conjunction of two mutually-necessary facts *)
+Lemma initStateValidDom s :
+  uniq s -> dom (initState' s) =i s /\ valid (initState' s).
+Proof.
+elim: s => /=[|a s']; first by rewrite valid_unit dom0.
+move => IH.
+move/andP => [H_ni H_u].
+move/IH: H_u => [H1 H2] {IH}.
+split; last first.
+- case: validUn; rewrite ?um_validPt ?H2//.
+  move=>k; rewrite um_domPt inE=>/eqP Z; subst k.
+  rewrite H1.
+  by move/negP: H_ni.
+- move=>z; rewrite domUn !inE !um_domPt !inE.
+  rewrite H1.
+  case validUn.
+  * by move/negP => H_v; case: H_v; rewrite um_validPt.
+  * by move/negP.
+  * move => k.
+    rewrite H1.
+    rewrite um_domPt inE=>/eqP H_eq.
+    rewrite -H_eq => H_in.
+    by move/negP: H_ni.
+  * move => Hv1 Hv2 H_d.
+    by rewrite eq_sym.
+Qed.
+
+Lemma valid_initState' s : uniq s -> valid (initState' s).
+Proof. by move => H_u; case: (initStateValidDom H_u). Qed.
+
+Lemma dom_initState' s : uniq s -> dom (initState' s) =i s.
+Proof. by move => H_u; case: (initStateValidDom H_u). Qed.
+
+(* ------------------*)
+(* TRANSITION SYSTEM *)
+(* ------------------*)
+
+Definition initState := initState' (enum Address).
+
+Definition PacketSoup := seq Packet.
+
+Record World :=
+  mkW {
+    localState : StateMap;
+    inFlightMsgs : PacketSoup;
+    consumedMsgs : PacketSoup;
+  }.
+
+Definition holds (n : Address) (w : World) (cond : State -> Prop) :=
+  forall (st : State),
+    find n (localState w) = Some st -> cond st.
+
+Definition Coh (w : World) :=
+  [/\ valid (localState w),
+     forall (n : Address),
+       holds n w (fun st => id st == n),
+     forall (n : Address),
+       holds n w (fun st => valid (blockTree st)),
+     forall (n : Address),
+       holds n w (fun st => validH (blockTree st)),
+     forall (n : Address),
+       holds n w (fun st => has_init_block (blockTree st)) &
+     forall (n : Address),
+       holds n w (fun st => uniq (peers st))
+  ].
+
+Record Qualifier := Q { ts: Timestamp; allowed: Address; }.
+
+(* Don't you worry about uniqueness of the messages? *)
+Inductive system_step (w w' : World) (q : Qualifier) : Prop :=
+| Idle of Coh w /\ w = w'
+
+| Deliver (p : Packet) (st : State) of
+      Coh w & (dst p) = allowed q &
+      p \in inFlightMsgs w &
+      find (dst p) (localState w) = Some st &
+      let: (st', ms) := procMsg st (src p) (msg p) (ts q) in
+      w' = mkW (upd (dst p) st' (localState w))
+               (seq.rem p (inFlightMsgs w) ++ ms)
+               (rcons (consumedMsgs w) p)
+
+| Intern (proc : Address) (t : InternalTransition) (st : State) of
+      Coh w & proc = allowed q &
+      find proc (localState w) = Some st &
+      let: (st', ms) := (procInt st t (ts q)) in
+      w' = mkW (upd proc st' (localState w))
+               (ms ++ (inFlightMsgs w))
+               (consumedMsgs w).
+
+Definition Schedule := seq Qualifier.
+
+Fixpoint reachable' (s : Schedule) (w w' : World) : Prop :=
+  if s is (ins :: insts)
+  then exists via, reachable' insts w via /\ system_step via w' ins
+  else w = w'.
+
+Definition reachable (w w' : World) :=
+  exists s, reachable' s w w'.
+
+Definition initWorld := mkW initState [::] [::].
+
+Ltac Coh_step_case n d H F :=
+  case B: (n == d);
+  do? [by move=>F; move: (H n _ F) |
+    case: ifP; last done
+  ]; move=>_ [] <-.
+
+Lemma holds_Init_state : forall (P : State -> Prop) n, P (Init n) ->
+  holds n {| localState := initState; inFlightMsgs := [::]; consumedMsgs := [::] |} (fun st : State => P st).
+Proof.
+move => P n H_P; rewrite /initState.
+have H_in: n \in enum Address by rewrite mem_enum.
+have H_un: uniq (enum Address) by apply enum_uniq.
+move: H_in H_un; elim: (enum Address) => //=.
+move => a s IH; rewrite inE; move/orP; case.
+* move/eqP => H_eq /=.
+  rewrite H_eq; move/andP => [H_in H_u].
+  rewrite /holds /= => st; rewrite gen_findPtUn; first by case => H_i; rewrite -H_i -H_eq.
+  by case: validUn; rewrite ?um_validPt ?valid_initState'//;
+   move=>k; rewrite um_domPt !inE=>/eqP <-;
+   rewrite dom_initState' //; move/negP: H_in.
+* move => H_in; move/andP => [H_ni H_u].
+  have H_neq: n <> a by move => H_eq; rewrite -H_eq in H_ni; move/negP: H_ni.
+  move: H_in; move/IH {IH} => IH.
+  have H_u' := H_u.
+  move: H_u'; move/IH {IH}.
+  rewrite /holds /= => IH st; rewrite findUnL.
+  + case: ifP; last by move => H_in H_f; exact: IH.
+    by rewrite um_domPt inE eq_sym; move/eqP.
+  + by case: validUn; rewrite ?um_validPt ?valid_initState'//;
+     move=>k; rewrite um_domPt !inE=>/eqP <-;
+     rewrite dom_initState' //; move/negP: H_ni.
+Qed.
+
+Lemma Coh_init : Coh initWorld.
+Proof.
+rewrite /initWorld/localState/=; split.
+- apply: valid_initState'.
+  exact: enum_uniq.
+- by move => n; exact: holds_Init_state.
+- move => n; apply: holds_Init_state.
+  by rewrite /blockTree /= um_validPt.
+- move => n; apply: holds_Init_state.
+  rewrite/validH/blockTree /= => h b H.
+  by move: (um_findPt_inv H); elim=>->->.
+- move => n; apply: holds_Init_state.
+  by rewrite/has_init_block/blockTree um_findPt.
+- move => n; exact: holds_Init_state.
+Qed.
+
+Lemma procMsg_id_constant (s1 : State) from (m : Message) (ts : Timestamp) :
+    id s1 = id (procMsg s1 from m ts).1.
+Proof.
+case: s1 from m ts=>n1 p1 b1 t1 from []=>//=??; case:ifP => //=.
+move/eqP => H_neq; case: ifP; move/eqP => //= H_eq.
+by case ohead.
+Qed.
+
+Lemma procInt_id_constant : forall (s1 : State) (t : InternalTransition) (ts : Timestamp),
+    id s1 = id (procInt s1 t ts).1.
+Proof.
+case=> n1 p1 b1 t1 [] =>// ts; simpl.
+case hP: genProof => //; case vP: (VAF _)=>//.
+case tV: (tx_valid_block _ _)=>//.
+Qed.
+
+Lemma btExtendV bt b : valid bt = valid (btExtend bt b).
+Proof.
+rewrite /btExtend; case: ifP=>//N.
+by rewrite gen_validPtUn/= N andbC.
+Qed.
+
+Lemma procMsg_valid :
+   forall (s1 : State) from (m : Message) (ts : Timestamp),
+    valid (blockTree s1) -> valid (blockTree (procMsg s1 from  m ts).1).
+Proof.
+move=> s1 from  m ts.
+case Msg: m=>[b|||];
+destruct s1; rewrite/procMsg/=; do?by [|move: (btExtendV blockTree0 b)=><-].
+case:ifP => //=.
+move/eqP => H_neq; case: ifP; move/eqP => //= H_eq H_v.
+by case ohead.
+Qed.
+
+Lemma procInt_valid :
+  forall (s1 : State) (t : InternalTransition) (ts : Timestamp),
+    valid (blockTree s1) = valid (blockTree (procInt s1 t ts).1).
+Proof.
+move=>s1 t ts.
+case Int: t; destruct s1; rewrite/procInt/=; first by [].
+case: (genProof _); last done.
+move=>Pf; case: (VAF _ _ _); last done.
+case tV: (tx_valid_block _ _)=>//.
+by rewrite/blockTree/=; apply btExtendV.
+Qed.
+
+Lemma btExtendH bt b : valid bt -> validH bt -> validH (btExtend bt b).
+Proof.
+move=>V H z c; rewrite /btExtend.
+case: ifP=>X; first by move/H.
+rewrite findUnL ?gen_validPtUn ?V ?X//.
+case: ifP=>Y; last by move/H.
+rewrite um_domPt inE in Y; move/eqP: Y=>Y; subst z.
+by rewrite um_findPt; case=>->.
+Qed.
+
+Lemma procMsg_validH :
+   forall (s1 : State) from  (m : Message) (ts : Timestamp),
+     valid (blockTree s1) -> validH (blockTree s1) ->
+     validH (blockTree (procMsg s1 from  m ts).1).
+Proof.
+move=> s1 from  m ts.
+case Msg: m=>[b|||];
+destruct s1; rewrite/procMsg/=; do? by []; do? by case: ifP => //=.
+- by move=>v vh; apply btExtendH.
+- move=>v vh; case: ifP => //=; move/eqP => H_neq; case: ifP; move/eqP => //= H_eq.
+  by case ohead.
+Qed.
+
+Lemma procInt_validH :
+   forall (s1 : State) (t : InternalTransition) (ts : Timestamp),
+     valid (blockTree s1) -> validH (blockTree s1) ->
+     validH (blockTree (procInt s1 t ts).1).
+Proof.
+move=>s1 t ts v vh.
+case Int: t; destruct s1; rewrite/procInt/=; first by [].
+case: (genProof _); last done.
+move=>Pf; case: (VAF _ _ _); last done.
+case tV: (tx_valid_block _ _)=>//.
+by rewrite/blockTree/=; apply btExtendH.
+Qed.
+
+Lemma btExtendIB bt b :
+  valid bt -> validH bt -> has_init_block bt ->
+  has_init_block (btExtend bt b).
+Proof.
+move=>V H; rewrite /btExtend/has_init_block=>Ib.
+case: ifP=>X; first done.
+rewrite findUnL ?gen_validPtUn ?V ?X//.
+case: ifP=>Y; last done.
+rewrite um_domPt inE in Y; move/eqP: Y=>Y.
+by specialize (hashB_inj Y)=><-; rewrite Y um_findPt.
+Qed.
+
+Lemma procMsg_has_init_block:
+   forall (s1 : State) from (m : Message) (ts : Timestamp),
+     valid (blockTree s1) -> validH (blockTree s1) ->
+     has_init_block (blockTree s1) ->
+     has_init_block (blockTree (procMsg s1 from m ts).1).
+Proof.
+move=> s1 from  m ts.
+case Msg: m=>[b|||];
+destruct s1; rewrite/procMsg/=; do? by []; do? by case:ifP.
+- by apply btExtendIB.
+- move=>v vh; case: ifP => //=; move/eqP => H_neq; case: ifP; move/eqP => //= H_eq.
+  by case ohead.
+Qed.
+
+Lemma procInt_has_init_block :
+   forall (s1 : State) (t : InternalTransition) (ts : Timestamp),
+     valid (blockTree s1) -> validH (blockTree s1) ->
+     has_init_block (blockTree s1) ->
+     has_init_block (blockTree (procInt s1 t ts).1).
+Proof.
+move=>s1 t ts v vh.
+case Int: t; destruct s1; rewrite/procInt/=; first by [].
+case: (genProof _); last done.
+move=>Pf; case: (VAF _ _ _); last done.
+case tV: (tx_valid_block _ _)=>//.
+by apply btExtendIB.
+Qed.
+
+Lemma procMsg_peers_uniq :
+  forall (s1 : State) from  (m : Message) (ts : Timestamp),
+    let: s2 := (procMsg s1 from m ts).1 in
+    uniq (peers s1) -> uniq (peers s2).
+Proof.
+case=> n1 p1 b1 t1 from; case; do? by []; simpl.
+move=>s _ U; case: ifP => //=.
+move/eqP => H_eq; case: ifP; move/eqP => //= H_eq'.
+by case ohead.
+Qed.
+
+Lemma procInt_peers_uniq :
+  forall (s1 : State) (t : InternalTransition) ts, let: s2 := (procInt s1 t ts).1 in
+    uniq (peers s1) -> uniq (peers s2).
+Proof.
+move=>s1 t ts; case: s1=>n prs bt txp; rewrite /peers/procInt=>Up.
+case: t=>//; case hP: (genProof _)=>//; case vP: (VAF _)=>//.
+case tV: (tx_valid_block _ _)=>//.
+Qed.
+
+Lemma Coh_step w w' q:
+  system_step w w' q -> Coh w'.
+Proof.
+move=>S; (have: system_step w w' q by done)=>S'.
+case: S'.
+(* Idle *)
+by case=>Cw <-.
+(* Deliver *)
+- move=> p st [H1 H2 H3 H4 H5 H6] _ iF sF; case P: (procMsg _ _ _)=>[st' ms].
+  move=>->; split;
+    do? [rewrite /holds/localState; move=> n stN; rewrite findU=>/=].
+  + rewrite /localState validU=>/=; apply H1.
+  + Coh_step_case n (dst p) H2 F; move/eqP: (H2 (dst p) _ sF)=>Id.
+    move: (procMsg_id_constant st (src p) (msg p) (ts q)).
+    by move/eqP in B; subst n; rewrite Id=>->; rewrite P.
+  + Coh_step_case n (dst p) H3 F; move: (H3 (dst p) _ sF)=>V.
+    by move: (procMsg_valid (src p) (msg p) (ts q) V); rewrite P.
+  + Coh_step_case n (dst p) H4 F;
+    move: (H3 (dst p) _ sF)=>V; move: (H4 (dst p) _ sF)=>VH;
+    rewrite [procMsg _ _ _ _] surjective_pairing in P; case: P=><- _;
+    by apply procMsg_validH.
+  + Coh_step_case n (dst p) H5 F.
+    move: (H3 (dst p) _ sF)=>V; move: (H4 (dst p) _ sF)=>VH;
+    rewrite [procMsg _ _ _ _] surjective_pairing in P; case: P=><- _;
+    by move: (H5 (dst p) _ sF); apply procMsg_has_init_block.
+  + Coh_step_case n (dst p) H6 F.
+    move: (H3 (dst p) _ sF)=>V; move: (H4 (dst p) _ sF)=>VH;
+    rewrite [procMsg _ _ _ _] surjective_pairing in P; case: P=><- _.
+    by move: (H6 (dst p) _ sF); apply procMsg_peers_uniq.
+
+(* Intern *)
+- move=> proc t st [H1 H2 H3 H4 H5 H6] _ sF. case P: (procInt _ _ _)=>[st' ms].
+  move=>->; split;
+    do? [rewrite /holds/localState; move=> n stN; rewrite findU=>/=].
+  + rewrite /localState validU=>/=; apply H1.
+  + Coh_step_case n proc H2 F; move/eqP: (H2 proc _ sF)=>Id.
+    move: (procInt_id_constant st t (ts q)).
+    by move/eqP in B; subst n; rewrite Id=>->; rewrite P.
+  + Coh_step_case n proc H3 F; move: (H3 proc _ sF)=>V.
+    by move: (procInt_valid st t (ts q)); rewrite P/==><-.
+  + Coh_step_case n proc H4 F;
+    move: (H3 proc _ sF)=>V; move: (H4 proc _ sF)=>VH;
+    rewrite [procInt _ _ _] surjective_pairing in P; case: P=><- _;
+    by apply procInt_validH.
+  + Coh_step_case n proc H5 F.
+    move: (H3 proc _ sF)=>V; move: (H4 proc _ sF)=>VH;
+    rewrite [procInt _ _ _] surjective_pairing in P; case: P=><- _;
+    by move: (H5 proc _ sF); apply procInt_has_init_block.
+  + Coh_step_case n proc H6 F.
+    move: (H3 proc _ sF)=>V; move: (H4 proc _ sF)=>VH;
+    rewrite [procInt _ _ _] surjective_pairing in P; case: P=><- _.
+    by move: (H6 proc _ sF); apply procInt_peers_uniq.
+Qed.
+
+(* Stepping does not remove or add nodes *)
+Lemma step_nodes w w' q :
+  system_step w w' q ->
+  dom (localState w) =i dom (localState w').
+Proof.
+case: w w'=>sm f c [sm'] f' c'; case=>/=; first by case=>C; case=>->/=.
+- move=>p st1 C iq pf F; case: (procMsg st1 (src p) (msg p))=>st2 ms[]->{sm'}Z1 Z2.
+  subst f' c'=>z; rewrite domU inE/=; case: ifP=>///eqP->{z}.
+  by move/find_some: F->; case: C.
+move=>p t st1 C iq F; case: (procInt st1 t)=>st2 ms[]->{sm'}Z1 Z2.
+subst f' c'=>z; rewrite domU inE/=; case: ifP=>///eqP->{z}.
+by move/find_some: F->; case: C.
+Qed.
+
+Lemma steps_nodes (w w' : World):
+  reachable w w' ->
+  dom (localState w) =i dom (localState w').
+Proof.
+move=>[sch] R. elim: sch w' R=>/=[w'->|q qs Hi w' [via] [R S]]//z.
+by move: (Hi via R)->; rewrite (step_nodes S).
+Qed.
+
+Inductive local_step (s1 s2 : State) : Prop :=
+| IdleStep of s1 = s2
+| RcvMsgStep f m ts of (s2 = (procMsg s1 f m ts).1)
+| IntTStep t ts of (s2 = (procInt s1 t ts).1).
+
+Lemma system_step_local_step w w' q:
+  forall (n : Address) (st st' : State),
+    system_step w w' q ->
+    find n (localState w) = Some st ->
+    find n (localState w') = Some st' ->
+    local_step st st'.
+Proof.
+move=> n st st'.
+case.
+(* Idle *)
+- by move=>[] cW<-->[]->; constructor 1.
+(* Deliver *)
+- move=> p old_st cW _ pIF osF.
+  case P: (procMsg _ _ _). case: w'. move=> sm' f' c'. case.
+  move=> A B C. subst sm' f' c'. move=> sF. rewrite /localState findU=>/=.
+  case B: (n == dst p); last first.
+    (* n != dst p -- node n is Idle => st st' *)
+    + move=> F. rewrite F in sF. case: sF=>stEq. rewrite stEq. by constructor 1.
+    (* When n == dst p, notice that st = old_st
+     * and st and st' are related by procMsg *)
+    + move/eqP in B. rewrite -B in osF. rewrite sF in osF. case: osF=>->.
+      case: ifP; last first.
+        by move=> _ con; contradict con.
+        move=> _ sEq. case: sEq=>stEq. rewrite stEq in P.
+        by constructor 2 with (src p) (msg p) (ts q); rewrite P.
+(* Intern *)
+- move=> proc t old_st cW _ osF.
+  case P: (procInt _ _ _). case: w'. move=> sm' f' c'. case.
+  move=> A B C. subst sm' f' c'. move=> sF. rewrite /localState findU=>/=.
+  case B: (n == proc); last first.
+    (* n != proc -- node n is Idle => st st' *)
+    + move=> F. rewrite F in sF. case: sF=>stEq. rewrite stEq. by constructor 1.
+    (* n == proc => update; akin to Deliver *)
+    + move/eqP in B. rewrite -B in osF. rewrite sF in osF. case: osF.
+      move=> stEq. rewrite -stEq in P. clear stEq old_st.
+      case: ifP; last first.
+        by move=> _ con; contradict con.
+        move=> _ sEq. case: sEq=> stEq. rewrite stEq in P.
+        by constructor 3 with t (ts q); rewrite P.
+Qed.
+
+Lemma no_change_still_holds (w w' : World) (n : Address) q st cond:
+  find n (localState w) = Some st ->
+  holds n w cond ->
+  system_step w w' q ->
+  find n (localState w') = Some st ->
+  holds n w' cond.
+Proof.
+move=>f h S sF st' s'F; rewrite s'F in sF; case: sF=>->.
+by move: (h st f).
+Qed.
+
+Lemma no_change_has_held (w w' : World) (n : Address) q st cond:
+  find n (localState w) = Some st ->
+  system_step w w' q->
+  holds n w' cond ->
+  find n (localState w') = Some st ->
+  holds n w cond.
+Proof.
+move=> f S h sF st' s'F.
+by rewrite f in s'F; case: s'F=><-; move: (h st sF).
+Qed.
